crdt_specs2.thy
@@ -1,5 +1,6 @@
 theory crdt_specs2
   imports crdt_specs
+ "fuzzyrule.fuzzyrule"
 begin
 
 section "CRDT Specifications Part 2"
@@ -23,6 +24,32 @@ type_synonym ('op, 'opn, 'res) ccrdtSpec =
 
 text "There is a mapping between the composable CRDT specs above and the original specifications:"
 
+definition 
+"extract_op c_calls c \<equiv>  case c_calls c of Some (Call op r) \<Rightarrow> op"
+
+(* TODO utils *)
+lemma option_bind_def:
+"(x \<bind> f) = (case x of None \<Rightarrow> None | Some a \<Rightarrow> f a)"
+  by (metis bind.bind_lunit bind_eq_None_conv option.case_eq_if option.exhaust_sel)
+
+definition is_reverse :: "('a \<rightharpoonup> 'b) \<Rightarrow> ('b \<Rightarrow> 'a) \<Rightarrow> bool" where
+"is_reverse f_in f_out \<equiv> 
+  (\<forall>x y. f_in x \<triangleq> y \<longrightarrow> f_out y = x)
+  \<and> (\<forall>x.  f_in (f_out x) \<triangleq> x)"
+
+lemma is_reverse_1:
+  assumes "is_reverse f_in f_out"
+    and "f_in x \<triangleq> y"
+  shows "f_out y = x"
+  by (meson assms is_reverse_def)
+
+
+lemma is_reverse_2:
+  assumes "is_reverse f_in f_out"
+  shows "f_in (f_out x) \<triangleq> x"
+  by (meson assms is_reverse_def)
+
+
 (* TODO
 so far the relation is only without nesting (for identity mapping.
 Must add the mapping to both sides of the equation
@@ -30,12 +57,22 @@ left through transforming the context, right through C directly
 
 best to prove equivalence for the map first and see what is required
  *)
-definition crdt_spec_rel :: "('op, 'res) crdtSpec \<Rightarrow> ('op, 'op, 'res) ccrdtSpec \<Rightarrow> bool" where
+definition crdt_spec_rel :: "('opn, 'res) crdtSpec \<Rightarrow> ('op, 'opn, 'res) ccrdtSpec \<Rightarrow> bool" where
 "crdt_spec_rel spec cspec \<equiv>
-(\<forall>ctxt op r. 
-spec op ctxt r \<longleftrightarrow> cspec (dom (calls ctxt)) (\<lambda>c. case calls ctxt c of Some (Call op r) \<Rightarrow> op) (happensBefore ctxt) id op r)
+\<forall>C_in::'op \<rightharpoonup> 'opn. \<forall>C_out::'opn \<Rightarrow> 'op.
+  is_reverse C_in C_out
+  \<longrightarrow> 
+  (\<forall>ctxt (outer_op::'op) (op::'opn) r Cs. 
+   C_in outer_op \<triangleq> op
+    \<longrightarrow>
+       (spec op (sub_context C_in Cs ctxt) r
+    \<longleftrightarrow> cspec (dom (calls ctxt) \<inter> Cs) (extract_op (calls ctxt))  (happensBefore ctxt) C_out op r))
 
 "
+
+lemmas use_crdt_spec_rel = crdt_spec_rel_def[unfolded atomize_eq, THEN iffD1, rule_format]
+lemmas use_crdt_spec_rel1 = crdt_spec_rel_def[unfolded atomize_eq, THEN iffD1, rule_format, THEN iffD1]
+lemmas use_crdt_spec_rel2 = crdt_spec_rel_def[unfolded atomize_eq, THEN iffD1, rule_format, THEN iffD2]
 
 
 subsection "Register"
@@ -74,15 +111,16 @@ lemma
   unfolding crdt_spec_rel_def
 proof (intro allI impI)
 
-  show "lww_register_spec initial op ctxt r =
-       lww_register_spec' initial (dom (calls ctxt)) (\<lambda>c. case calls ctxt c of None \<Rightarrow> ??? | Some (Call op r) \<Rightarrow> op) (happensBefore ctxt)
-        id op r" (is ?g)
-    for ctxt op r
+  show "lww_register_spec initial op (sub_context C_in Cs ctxt) r = lww_register_spec' initial (dom (calls ctxt) \<inter> Cs) (extract_op (calls ctxt)) (happensBefore ctxt) C_out op r"
+    if c0: "is_reverse C_in C_out"
+      and c1: "C_in outer_op \<triangleq> op"
+    for  C_in C_out ctxt outer_op op r Cs
   proof -
 
-    have h1: "(latest_assignments' (dom (calls ctxt)) (\<lambda>c. case calls ctxt c of None \<Rightarrow> ??? | Some (Call op r) \<Rightarrow> op) (happensBefore ctxt) id)
+(*
+    have h1: "(latest_assignments' (dom (calls ctxt)) (extract_op (calls ctxt)) (happensBefore ctxt) id)
     = {(x,y). latestAssignments ctxt x \<triangleq> y}"
-      apply (auto simp add: latest_assignments'_def latestAssignments_def latestAssignments_h_def split: call.splits)
+      apply (auto simp add: latest_assignments'_def extract_op_def latestAssignments_def latestAssignments_h_def split: call.splits)
          apply (auto split: option.splits call.splits registerOp.splits if_splits)
       done
 
@@ -95,13 +133,13 @@ proof (intro allI impI)
           = firstValue initial (latestAssignments ctxt)"
       apply (auto simp add: firstValue'_def firstValue_def h2)
       by (smt dom_def emptyE mem_Collect_eq option.exhaust option.sel some_well_order_includes_all some_well_order_is_wo_rel wo_rel.minim_in)
+*)
 
 
-
-    show ?g
+    show " lww_register_spec initial op (sub_context C_in Cs ctxt) r =
+    lww_register_spec' initial (dom (calls ctxt) \<inter> Cs) (extract_op (calls ctxt)) (happensBefore ctxt) C_out op r"
       apply (auto simp add: lww_register_spec_def lww_register_spec'_def split: registerOp.splits)
-      apply (auto simp add: h1 h3)
-      done
+      sorry
   qed
 qed
 
@@ -132,14 +170,154 @@ definition
 "restrict_calls vis op C k \<equiv>
 {c\<in>vis. \<exists>u. op c = C (NestedOp k u) }"
 
-definition
+definition map_spec' :: "
+      (callId set  \<Rightarrow> (callId \<Rightarrow>'op) \<Rightarrow> callId rel \<Rightarrow> (('k, 'opn) mapOp \<Rightarrow> 'op) \<Rightarrow> 'k \<Rightarrow> callId set) 
+    \<Rightarrow> (bool \<Rightarrow> 'r)
+    \<Rightarrow> ('op, 'opn::crdt_op, 'r) ccrdtSpec
+    \<Rightarrow> ('op, ('k, 'opn) mapOp, ('r::default)) ccrdtSpec" where
 "map_spec' deleted_calls from_bool nestedSpec vis op hb C oper res \<equiv>
   case oper of
     DeleteKey k \<Rightarrow> res = default
-  | KeyExists k \<Rightarrow> res = from_bool (\<exists>c\<in>vis. \<exists>upd_op. op c \<triangleq> NestedOp k upd_op \<and> is_update upd_op \<and>  c \<notin> deleted_calls vis op hb C k)
+  | KeyExists k \<Rightarrow> res = from_bool (\<exists>c\<in>vis. \<exists>upd_op. op c = C (NestedOp k upd_op) \<and> is_update upd_op \<and>  c \<notin> deleted_calls vis op hb C k)
   | NestedOp k nested_op \<Rightarrow>
      nestedSpec (restrict_calls vis op C k - deleted_calls vis op hb C k) op hb (\<lambda>x. C (NestedOp k x)) nested_op res
 "
 (* Needed for example: structs, set_rw, map_rw *)
+
+
+
+
+lemma subcontext_calls:
+  assumes in_out: "is_reverse C_in C_out"
+  shows "(calls (sub_context C_in Cs ctxt) c \<triangleq> Call op r)
+     \<longleftrightarrow> (calls ctxt c \<triangleq> Call (C_out op) r \<and> c\<in>Cs \<and> C_in (C_out op) \<triangleq> op)"
+
+  by (auto simp add:   sub_context_def restrict_ctxt_op_def restrict_ctxt_def fmap_map_values_def ctxt_restrict_calls_def restrict_map_def option_bind_def split: option.splits call.splits,
+      (simp add: in_out[simplified is_reverse_def])+)
+
+lemma subcontext_of_subcontext_collapse:
+"sub_context C_inA CsA (sub_context C_inB CsB ctxt)
+= sub_context (\<lambda>x. C_inB x \<bind> C_inA) (CsA \<inter> CsB) ctxt"
+  by (auto simp add: sub_context_def restrict_ctxt_op_def restrict_ctxt_def restrict_hb_def 
+      fmap_map_values_def ctxt_restrict_calls_def restrict_map_def option_bind_def
+      restrict_relation_def
+      intro!: ext split: option.splits call.splits)
+
+  
+
+
+lemma map_spec_rel:
+  fixes nestedSpec :: "('opn::crdt_op, 'res::default) crdtSpec"
+    and nestedSpec' :: "('op, 'opn, 'res) ccrdtSpec"
+    and deletedCalls :: "(('k, 'opn) mapOp, 'res) operationContext \<Rightarrow> 'k \<Rightarrow> callId set"
+    and deletedCalls' :: "callId set \<Rightarrow> (callId \<Rightarrow> 'op) \<Rightarrow> (callId \<times> callId) set \<Rightarrow> (('k, 'opn) mapOp \<Rightarrow> 'op) \<Rightarrow> 'k \<Rightarrow> callId set"
+  assumes nested_rel: "crdt_spec_rel nestedSpec nestedSpec'"
+and deletedCalls_rel: 
+    "\<And>ctxt C_in C_out Cs k. deleted_calls (sub_context C_in Cs ctxt) k
+        = deleted_calls' (dom (calls ctxt) \<inter> Cs) (extract_op (calls ctxt)) (happensBefore ctxt) C_out k"
+shows "crdt_spec_rel (map_spec deleted_calls from_bool nestedSpec) (map_spec' deleted_calls' from_bool nestedSpec') "
+  unfolding crdt_spec_rel_def
+proof (intro allI impI)
+
+  show "map_spec deleted_calls from_bool nestedSpec op (sub_context C_in Cs ctxt) r = map_spec' deleted_calls' from_bool nestedSpec' (dom (calls ctxt) \<inter> Cs) (extract_op (calls ctxt)) (happensBefore ctxt) C_out op r" (is "?l = ?r")
+    if is_rev: "is_reverse C_in C_out"
+      and op_def: "C_in outer_op \<triangleq> op"
+    for  C_in C_out ctxt outer_op op r Cs
+
+  proof -
+
+
+    show "?l = ?r"
+    proof (cases op)
+      case (NestedOp k nestedOp)
+
+
+       have h1: "(restrict_calls (dom (calls ctxt) \<inter> Cs) (extract_op (calls ctxt)) C_out k - deleted_calls' (dom (calls ctxt) \<inter> Cs) (extract_op (calls ctxt)) (happensBefore ctxt) C_out k) = 
+            {c \<in> dom (calls ctxt). c \<in> Cs \<and> (\<exists>u. extract_op (calls ctxt) c = C_out (NestedOp k u)) \<and> c \<notin> deleted_calls' (dom (calls ctxt) \<inter> Cs) (extract_op (calls ctxt)) (happensBefore ctxt) C_out k}
+              " 
+         by (auto simp add: restrict_calls_def)
+
+       have h2: "nestedSpec nestedOp
+         (sub_context (nested_op_on_key k) (- deleted_calls (sub_context C_in Cs ctxt) k) (sub_context C_in Cs ctxt))
+         r 
+          = ???"
+         thm use_crdt_spec_rel[OF nested_rel, 
+             where op=nestedOp 
+               and r=r
+               and C_in="\<lambda>x. C_in x \<bind> nested_op_on_key k"
+               and C_out="\<lambda>x. C_out (NestedOp k x)"]
+         sorry
+
+
+      show ?thesis 
+      proof (simp add: NestedOp h1 map_spec_def map_spec'_def subcontext_calls[OF is_rev] deletedCalls_rel subcontext_of_subcontext_collapse)
+
+        show " nestedSpec nestedOp
+         (sub_context (\<lambda>x. C_in x \<bind> nested_op_on_key k) (- deleted_calls (sub_context C_in Cs ctxt) k \<inter> Cs) ctxt) r =
+        nestedSpec'
+         {c \<in> dom (calls ctxt).
+          c \<in> Cs \<and>
+          (\<exists>u. extract_op (calls ctxt) c = C_out (NestedOp k u)) \<and>
+          c \<notin> deleted_calls' (dom (calls ctxt) \<inter> Cs) (extract_op (calls ctxt)) (happensBefore ctxt) C_out k}
+         (extract_op (calls ctxt)) (happensBefore ctxt) (\<lambda>x. C_out (NestedOp k x)) nestedOp r"
+        proof (subst use_crdt_spec_rel[OF nested_rel])        
+
+          show is_rev_combined: "is_reverse (\<lambda>x. C_in x \<bind> nested_op_on_key k) (\<lambda>x. C_out (NestedOp k x))"
+            by (auto simp add: is_reverse_def option_bind_def nested_op_on_key_def 
+                is_reverse_1[OF is_rev] is_reverse_2[OF is_rev] split: option.splits mapOp.splits)
+
+          show "(C_in (C_out (NestedOp k nestedOp)) \<bind> nested_op_on_key k) \<triangleq> nestedOp"
+            using is_rev_combined is_reverse_def by fastforce
+
+          have h1: "deleted_calls (sub_context C_in Cs ctxt) k
+              = deleted_calls' (dom (calls ctxt) \<inter> Cs) (extract_op (calls ctxt)) (happensBefore ctxt) C_out k"
+            by (rule deletedCalls_rel)
+            thm deletedCalls_rel
+
+          have "(dom (calls ctxt) \<inter> (- deleted_calls (sub_context C_in Cs ctxt) k \<inter> Cs)) 
+          = {c \<in> dom (calls ctxt). c \<in> Cs \<and> (\<exists>u. extract_op (calls ctxt) c = C_out (NestedOp k u)) \<and>
+                      c \<notin> deleted_calls' (dom (calls ctxt) \<inter> Cs) (extract_op (calls ctxt)) (happensBefore ctxt) C_out k}"
+            apply (auto simp add: h1)
+            apply (auto simp add: extract_op_def split: call.splits)
+            sorry
+
+
+          show "nestedSpec' 
+                  (dom (calls ctxt) \<inter> (- deleted_calls (sub_context C_in Cs ctxt) k \<inter> Cs)) 
+                  (extract_op (calls ctxt))
+                  (happensBefore ctxt) 
+                  (\<lambda>x. C_out (NestedOp k x)) 
+                  nestedOp 
+                  r =
+                  nestedSpec'
+                   {c \<in> dom (calls ctxt). c \<in> Cs \<and> (\<exists>u. extract_op (calls ctxt) c = C_out (NestedOp k u)) \<and>
+                      c \<notin> deleted_calls' (dom (calls ctxt) \<inter> Cs) (extract_op (calls ctxt)) (happensBefore ctxt) C_out k}
+                   (extract_op (calls ctxt)) (happensBefore ctxt) (\<lambda>x. C_out (NestedOp k x)) nestedOp r"
+
+
+          have "nestedSpec' (dom (calls ?ctxt) \<inter> ?Cs) (extract_op (calls ?ctxt)) (happensBefore ?ctxt) ?C_out ?op ?r"
+
+
+          thm use_crdt_spec_rel1[OF nested_rel]
+         apply (fuzzy_rule(noabs) use_crdt_spec_rel1)
+
+        sorry
+    next
+      case (KeyExists k)
+      then show ?thesis 
+        apply (auto simp add: map_spec_def map_spec'_def subcontext_calls[OF is_rev] deletedCalls_rel intro!: arg_cong[where f=from_bool])
+           apply (auto simp add:  extract_op_def split: option.splits call.splits)
+           apply (metis (no_types, lifting) Int_iff call.inject deletedCalls_rel domI domIff option.sel)
+          apply (meson deletedCalls_rel is_rev is_reverse_2)
+         apply (meson deletedCalls_rel is_rev is_reverse_2)
+        by (metis (no_types, lifting) Int_iff call.inject deletedCalls_rel domI domIff option.sel)
+    next
+      case (DeleteKey k)
+      then show ?thesis
+        by (auto simp add: map_spec_def map_spec'_def)
+    qed
+
+
+  qed
 
 end
